add distinct_vars and try to prove 3.9

src/Bohm_Tree.lean
@@ -12,19 +12,23 @@ universe u
 
 variable {Var : Type u}
 
+@[grind]
 inductive isHeadRedexApp : Term Var → Prop where
   | base N P₁ : isHeadRedexApp ((Term.abs N).app P₁)
   | step T Pₙ : isHeadRedexApp T → isHeadRedexApp (T.app Pₙ)
 
+@[grind]
 inductive isHeadRedex : Term Var → Prop where
   | base T : isHeadRedexApp T → isHeadRedex T
   | step T : isHeadRedex T → isHeadRedex (Term.abs T)
 
+@[grind]
 inductive isHeadNormalApp : Term Var → Prop where
   | base_free y : isHeadNormalApp (Term.fvar y)
   | base_bound n : isHeadNormalApp (Term.bvar n)
   | step T Pₙ : isHeadNormalApp T → isHeadNormalApp (T.app Pₙ)
 
+@[grind]
 inductive isHeadNormal : Term Var → Prop where
   | base T : isHeadNormalApp T → isHeadNormal T
   | step T : isHeadNormal T → isHeadNormal (Term.abs T)
@@ -49,9 +53,24 @@ lemma normal_or_redex (T : Term Var) : isHeadRedex T ∨ isHeadNormal T := by
       · cases ih1 ; left ; apply isHeadRedex.base ; apply isHeadRedexApp.step ; assumption
       · cases ih1 ; right ; apply isHeadNormal.base ; apply isHeadNormalApp.step ; assumption
 
+@[grind]
 inductive List.BetaEquiv : List (Term Var) → List (Term Var) → Prop where
   | base : [].BetaEquiv []
   | step as bs T₁ T₂ : T₁.BetaEquiv T₂ → as.BetaEquiv bs → (T₁ :: as).BetaEquiv (T₂ :: bs)
+
+lemma List.BetaEquivLength {L₁ L₂ : List (Term Var)} : L₁.BetaEquiv L₂ → L₁.length = L₂.length := by
+  induction L₁ generalizing L₂ <;> induction L₂
+  case nil.nil => simp
+  case nil.cons => grind
+  case cons.nil => grind
+  case cons.cons ih _ _ _ =>
+    simp_all
+    intro h
+    apply ih
+    grind
+
+lemma BetaEquivHelper {n} {L₁ L₂ : Vector (Term Var) n} (h : L₁.toList.BetaEquiv L₂.toList) : ∀ (x : Fin n), L₁[x] ≡β L₂[x] := by
+  sorry
 
 def bfvar (Var : Type u) := { v : Term Var // (exists n, v = Term.bvar n) ∨ (exists v', v = Term.fvar v') }
 
@@ -82,14 +101,13 @@ lemma BetaEquiv_of_BetaEquiv_abs (P Q : Term Var) (lc_P : P.LC) (lc_Q : Q.LC) (h
   case refl => sorry
   case trans R h₁ h₂ => sorry
 
-lemma destruct_BetaEquiv_nfoldAbs (n : ℕ) (P Q : Term Var) (lc_P : P.LC) (lc_Q : Q.LC) (h : nfoldAbs n P ≡β nfoldAbs n Q) : P ≡β Q := by
-  induction' n with n ih generalizing P Q
-  · exact h
-  · simp [nfoldAbs] at h
-    specialize ih _ _ _ _ h
-    · sorry
-    · sorry
-    · sorry
+lemma destruct_BetaEquiv_nfoldAbs (n : ℕ) (P Q : bfvar Var) (h : nfoldAbs n P.val ≡β nfoldAbs n Q.val) : P.val ≡β Q.val := by
+  induction n
+  case zero => exact h
+  case succ n ih =>
+    simp [nfoldAbs] at h ih
+    apply ih
+    sorry
 
 -- Reduction does not affect the number of leading abstractions, the head variable, or the number of arguments of the head-variable
 lemma reduction_preservation_fvar (n m : ℕ) (y z : bfvar Var) (Ps Qs : List (Term Var)) :
@@ -173,16 +191,22 @@ def böhm_tree_node {Var : Type u} [DecidableEq Var]: bfvar Var → List Var →
 def abs_vars_free {Var : Type u} [DecidableEq Var] (a : List Var) (b : List (Term Var)) : Prop :=
   ∀ x ∈ a, ∀ y ∈ b, x ∉ y.fv
 
+-- Whether all variables in the list are distinct
+@[simp]
+def distinct_vars [BEq Var] (l : List Var) : Prop :=
+  ∀ x (hx : x < l.length) y (hy : y < x), l[x]'hx != l[y]'(by trans x ; exact hy ; exact hx)
+
 -- Definition 3.7
 coinductive BT {Var : Type u} [DecidableEq Var] : Term Var → List Var → BöhmTree Var → Prop where
   | no_hnf (T : Term Var) (L : List Var) :
       ¬(exists n Ps y, hasAsHnf T n Ps y) →
       BT T L BöhmTree.no_hnf
-  | hnf (term : Term Var) (abs_vars : List Var) (term_base_var : bfvar Var) (term_apps : List (Term Var)) (subtrees : ULift (Fin term_apps.length) → BöhmTree Var) (L : List Var) :
-      hasAsHnf term abs_vars.length term_apps term_base_var →
-      abs_vars_free abs_vars (term_apps ++ L.map Term.fvar) →
-      (forall (m : ULift (Fin term_apps.length)), BT (nfoldOpen (abs_vars ++ L) term_apps[m.down]) (abs_vars ++ L) (subtrees m)) →
-      BT term L (BöhmTree.hnf term_apps.length abs_vars.length (böhm_tree_node term_base_var L) subtrees)
+  | hnf (term : Term Var) (abs_vars : List Var) (term_base_var : bfvar Var) (num_apps : ℕ) (term_apps : Vector (Term Var) num_apps) (subtrees : ULift (Fin num_apps) → BöhmTree Var) (L : List Var) :
+      hasAsHnf term abs_vars.length term_apps.toList term_base_var →
+      abs_vars_free abs_vars (term_apps.toList ++ L.map Term.fvar) →
+      distinct_vars abs_vars →
+      (forall (m : ULift (Fin num_apps)), BT (nfoldOpen (abs_vars ++ L) term_apps[m.down]) (abs_vars ++ L) (subtrees m)) →
+      BT term L (BöhmTree.hnf num_apps abs_vars.length (böhm_tree_node term_base_var L) subtrees)
 
 @[partial_fixpoint_monotone]
 theorem hnf_mono (t : bfvar Var) : monotone fun f ↦ BöhmTree.hnf 1 0 t fun _ ↦ f := by
@@ -199,27 +223,29 @@ theorem hnf_mono (t : bfvar Var) : monotone fun f ↦ BöhmTree.hnf 1 0 t fun _ 
 def BT_fvar (n : Var) : BöhmTree Var := .hnf 0 0 ⟨Term.fvar n, by simp⟩ (fun n ↦ .no_hnf)
 lemma BT_fvar_correct [DecidableEq Var] (n : Var) : BT (Term.fvar n) [] (BT_fvar n) := by
   unfold BT_fvar
-  apply BT.hnf _ [] ⟨Term.fvar n, by simp⟩ []
+  apply BT.hnf _ [] ⟨Term.fvar n, by simp⟩ 0 #v[]
   · simp [hasAsHnf]
     constructor
     · apply isHeadNormal.base
       apply isHeadNormalApp.base_free
     · apply Relation.EqvGen.refl
   · simp
-  . simp only [List.length_nil, List.append_nil, Fin.getElem_fin, IsEmpty.forall_iff]
+  · simp
+  . simp only [List.append_nil, Fin.getElem_fin, IsEmpty.forall_iff]
 
 -- BT of bound variable together with correctness proof
 def BT_bvar (n : ℕ) : BöhmTree Var := .hnf 0 0 ⟨Term.bvar n, by simp⟩ (fun n ↦ .no_hnf)
 lemma BT_bvar_correct [DecidableEq Var] (n : ℕ) : BT (@Term.bvar Var n) [] (BT_bvar n) := by
   unfold BT_bvar
-  apply BT.hnf _ [] ⟨Term.bvar n, by simp⟩ []
+  apply BT.hnf _ [] ⟨Term.bvar n, by simp⟩ 0 #v[]
   · simp [hasAsHnf]
     constructor
     · apply isHeadNormal.base
       apply isHeadNormalApp.base_bound
     · apply Relation.EqvGen.refl
   · simp
-  · simp only [List.length_nil, List.append_nil, Fin.getElem_fin, nfoldOpen, IsEmpty.forall_iff]
+  · simp
+  · simp only [List.append_nil, Fin.getElem_fin, nfoldOpen, IsEmpty.forall_iff]
 
 lemma exists_BT_for_term [DecidableEq Var] (M : Term Var) : ∃ L T, BT M L T := by
   induction M with
@@ -255,7 +281,7 @@ lemma omega_f_beta_f (f : Var) : (omega_f_free f).app (omega_f_free f) ≡β (Te
 
 lemma Ycombinator_tree [DecidableEq Var] [fresh : HasFresh Var] : BT (@Ycombinator Var) [] Ytree := by
   have f := fresh.fresh ∅
-  apply BT.hnf Ycombinator [f] ⟨Term.bvar 0, by simp⟩ [omega_f.app omega_f]
+  apply BT.hnf Ycombinator [f] ⟨Term.bvar 0, by simp⟩ 1 #v[omega_f.app omega_f]
   · constructor
     · apply isHeadNormal.step
       apply isHeadNormal.base
@@ -264,13 +290,14 @@ lemma Ycombinator_tree [DecidableEq Var] [fresh : HasFresh Var] : BT (@Ycombinat
     · simp [nfoldAbs, nfoldApp]
       nth_rw 1 [Ycombinator]
   · simp [omega_f]
+  · simp
   · intros m
     simp [nfoldOpen, Term.open', Term.openRec, omega_f]
     rw [←omega_f_free]
     apply BT.coinduct (fun term L tree ↦ tree = inf_Ytree ∧ L = [f] ∧ term = (omega_f_free f).app (omega_f_free f))
     · rintro term L tree ⟨prop_tree, prop_L, prop_term⟩
       right
-      use [], ⟨Term.fvar f, by simp⟩, [(omega_f_free f).app (omega_f_free f)], (λ _ ↦ inf_Ytree)
+      use [], ⟨Term.fvar f, by simp⟩, 1, #v[(omega_f_free f).app (omega_f_free f)], (λ _ ↦ inf_Ytree)
       simp
       constructor
       · simp [hasAsHnf, nfoldAbs, nfoldApp]
@@ -286,3 +313,16 @@ lemma Ycombinator_tree [DecidableEq Var] [fresh : HasFresh Var] : BT (@Ycombinat
         · simp [Term.open', Term.openRec, omega_f_free]
         · nth_rw 1 [inf_Ytree]
     · simp
+
+lemma BT_L_sub {Var} [DecidableEq Var] L₁ L₂ term tree (h_dis₁ : distinct_vars L₁) (h_dis₂ : distinct_vars L₂) : BT (Var:=Var) (nfoldOpen L₁ term) L₁ tree → BT (Var:=Var) (nfoldOpen L₂ term) L₂ tree := by
+  intros h
+  induction term
+  case bvar n =>
+    cases h
+    case no_hnf h =>
+      sorry
+    case hnf =>
+      sorry
+  case fvar x => sorry
+  case abs term ih => sorry
+  case app term₁ term₂ ih₁ ih₂ => sorry
